BasicRules.v
@@ -2,7 +2,7 @@ Require Import Toy.Imp.
 Require Import Toy.Language.
 Require Import Toy.Embeddings.
 
-Module BasicRules.
+Module BasicRulesSound.
 Import Validity Assertion_Shallow Denote_State Denote_Aexp Denote_Bexp Denote_Com.
 
 Theorem hoare_skip_sound : forall P, valid P CSkip P falsep falsep.
@@ -194,7 +194,189 @@ Proof.
   + simpl; tauto.
   + simpl; tauto.
 Qed. 
+
+Theorem hoare_consequence_sound : forall P P' Q Q' Rb Rb' Rc Rc' c,
+  derives P P' ->
+  valid P' c Q' Rb' Rc' ->
+  derives Q' Q ->
+  derives Rb' Rb ->
+  derives Rc' Rc ->
+  valid P c Q Rb Rc.
+Proof.
+  intros P P' Q Q' Rb Rb' Rc Rc' c HP Hc HQ HRb HRc.
+  unfold valid in *.
+  intros.
+  specialize (Hc st1 st2).
+  unfold derives in *.
+  specialize (HP st1); specialize (HQ st2).
+  specialize (HRb st2); specialize (HRc st2).
+  tauto.
+Qed.
+
+Theorem hoare_set_sound : forall P X e v,
+  derives P (eqp e v) ->
+  valid (andp P (safea e)) (CAss_set X e) (andp (eqp (AId X) v) (exp (subst_set P X))) falsep falsep.
+Proof.
+  unfold valid. intros.
+  unfold derives, eqp in H.
+  unfold andp, safea in H0.
+  destruct H0 as [? ?].
+  specialize (H st1 H0).
+  split.
+  { unfold not; simpl; tauto. }
+  split.
+  { intros.
+    unfold andp, eqp, exp, subst_set.
+    simpl in H2. destruct H2. split.
+    + simpl. rewrite H2. tauto.
+    + exists ((fst st1) X).
+      remember (store_update (fst st2) X (Some (fst st1 X))) as s'.
+      assert (forall X, s' X = (fst st1) X).
+      { destruct H3. intros Y.
+        unfold store_update in Heqs'.
+        subst s'.
+        destruct (Nat.eq_dec Y X).
+        - rewrite e0. tauto.
+        - specialize (H3 Y). specialize (H3 n). rewrite H3. tauto. } 
+      assert (store_update (fst st2) X (Some (fst st1 X)) = fst st1).
+      { eapply FunctionalExtensionality.functional_extensionality_dep.
+        subst. tauto. }
+      subst.
+      destruct H3. rewrite <- H6.
+      rewrite H5.
+      destruct st1 in *.
+      unfold fst, snd. tauto. }
+  split; simpl; tauto.
+Qed.
+
+Theorem hoare_load_sound : forall P X e p v,
+  derives P (andp (eqp e p) (storesv p v)) ->
+  valid (andp P (safea e)) (CAss_load X e) (andp (eqp (AId X) v) (exp (subst_load P X))) falsep falsep.
+Proof.
+  unfold valid. intros.
+  unfold derives, andp, eqp, storesv in H.
+  unfold andp, safea in H0. destruct H0.
+  specialize (H st1 H0). destruct H.
+  split.
+  { unfold not; intros. simpl in H3.
+    destruct (aeval e (fst st1)); try tauto.
+    inversion H; subst. rewrite H2 in H3; inversion H3. }
+  split.
+  { intros.
+    unfold andp, eqp, exp, subst_load.
+    split.
+    + simpl in *.
+      destruct (aeval e (fst st1)); try tauto.
+      destruct H3. inversion H; subst.
+      rewrite H3. tauto. 
+    + exists ((fst st1) X).
+      remember (store_update (fst st2) X (Some (fst st1 X))) as s'.
+      assert (forall X, s' X = (fst st1) X).
+      { intros Y. 
+        subst s'. unfold store_update.
+        destruct (Nat.eq_dec Y X).
+        - rewrite e0; tauto.
+        - simpl in H3.
+          destruct (aeval e (fst st1)); try tauto.
+          destruct H3 as [? [? ?]].
+          specialize (H4 Y n). tauto. }
+      assert (s' = fst st1).
+      { eapply FunctionalExtensionality.functional_extensionality_dep.
+        tauto. }
+      rewrite H5.
+      simpl in H3.
+      destruct (aeval e (fst st1)); try tauto.
+      destruct H3 as [? [? ?]].
+      rewrite <- H7.
+      destruct st1.
+      unfold fst, snd. tauto. }
+  split; simpl; tauto.
+Qed.
+
+Theorem hoare_store_sound : forall P e1 e2 p v,
+  derives P (andp (eqp e1 p) (eqp e2 v)) ->
+  valid (andp (sepcon P (saferef p)) (andp (safea e1) (safea e2))) (CAss_store e1 e2) (sepcon P (storesv p v)) falsep falsep.
+Proof.
+  unfold valid; intros.
+  unfold derives, andp, eqp in H.
+  unfold andp, sepcon, saferef, safea in H0.   
+  destruct H0 as [[st11 [st12 ?]] [? ?]].
+  destruct H0 as [? [? ?]].
+  split.
+  { unfold not; intros.
+    simpl in H5.
+    pose proof (H st11 H3).
+    destruct H6.
+    unfold join in H0.
+    destruct H0 as [? [? ?]].
+    rewrite H0 in H6, H7.
+    rewrite H8 in H6, H7.
+    rewrite H6, H7 in H5.
+    unfold join_heap in H9.
+    specialize (H9 p).
+    destruct H9 as [? | [? | ?]].
+    + destruct H9 as [p0 ?]. tauto.
+    + destruct H9 as [p0 ?]. destruct H9 as [? [? ?]].
+      rewrite H11 in H5. inversion H5.
+    + tauto. }
+  split.
+  { intros. 
+    unfold sepcon.
+    remember (fst st12, heap_update (snd st12) p (Some v)) as st22.
+    exists st11, st22.
+    simpl in H5.
+    unfold join in H0.
+    destruct H0 as [? [? ?]].
+    specialize (H st11 H3).
+    destruct H.
+    rewrite H0, H6 in H.
+    rewrite H0, H6 in H8.
+    rewrite H, H8 in H5.
+    destruct H5 as [? [? [? ?]]].
+    split.
+    { unfold join.
+      rewrite Heqst22 at 1 2.
+      simpl fst.
+      split; try tauto.
+      rewrite H6. split; try tauto.
+      unfold join_heap in *.
+      intros p0; specialize (H7 p0).
+      destruct H7 as [? | [? | ?]].
+      + left.
+        subst st22; unfold heap_update.
+        unfold snd at 2.
+        destruct (Z.eq_dec p p0).
+        { subst p0; destruct H7 as [v0 [? [? ?]]]; tauto. }
+        destruct H7 as [v0 ?].
+        exists v0.
+        split; try split; try tauto.
+        specialize (H10 p0 n).
+        rewrite H10. tauto.
+      + right; left.
+        destruct H7 as [v0 ?].
+        subst st22; unfold heap_update.
+        unfold snd at 2.
+        destruct (Z.eq_dec p p0).
+        - subst p0; exists v.
+          split; try split; try tauto.
+        - exists v0.
+          split; try split; try tauto.
+          specialize (H10 p0 n).
+          rewrite H10. tauto.
+      + right; right.
+        subst st22; unfold heap_update.
+        unfold snd at 2.
+        destruct (Z.eq_dec p p0).
+        { subst p0. tauto. }
+        specialize (H10 p0 n).
+        rewrite H10. tauto. }
+    split; try tauto.
+    subst st22.
+    unfold storesv, heap_update.
+    unfold snd at 1.
+    destruct (Z.eq_dec p p); try tauto. }
+  split; simpl; tauto.
+Qed.
+
+End BasicRulesSound.
         
-
-
-
